src/Lab1/StatDbImpl.v
@@ -12,35 +12,35 @@ Require Import StatDbAPI.
   *)
 
 
-Module StatDB (v : VarsAPI) <: StatDbAPI.
-
   Import ListNotations.
 
-  Definition add (v : nat) : proc unit :=
-    sum <- v.read VarSum;
-    count <- v.read VarCount;
-    _ <- v.write VarSum (sum + v);
-    _ <- v.write VarCount (count + 1);
+  Definition add (v : nat) : proc VariablesAPI.opT unit :=
+    sum <- Op _ _ (Read VarSum);
+    count <- Op _ _ (Read VarCount);
+    _ <- Op _ _ (Write VarSum (sum + v));
+    _ <- Op _ _ (Write VarCount (count + 1));
     Ret tt.
 
   (** ** Exercise : complete the implementation of mean *)
-  Definition mean : proc (option nat) :=
+  Definition mean : proc VariablesAPI.opT (option nat) :=
   (* SOL *)
-    count <- v.read VarCount;
+    count <- Op _ _ (Read VarCount);
     if count == 0 then
       Ret None
     else
-      sum <- v.read VarSum;
+      sum <- Op _ _ (Read VarSum);
       Ret (Some (sum / count)).
   (* END *)
   (* STUB:   Ret None. *)
 
+(*
   Definition init' : proc InitResult :=
     _ <- v.write VarCount 0;
     _ <- v.write VarSum 0;
     Ret Initialized.
 
   Definition init := then_init v.init init'.
+*)
 
   (** ** Exercise : complete the implementation of the abstraction function: *)
   Definition statdb_abstraction (vars_state : VariablesAPI.State) (statdb_state : StatDbAPI.State) : Prop :=
@@ -50,10 +50,8 @@ Module StatDB (v : VarsAPI) <: StatDbAPI.
   (* END *)
   (* STUB:   True. *)
 
-  Definition abstr : Abstraction StatDbAPI.State :=
-    abstraction_compose
-      v.abstr
-      {| abstraction := statdb_abstraction |}.
+  Definition abs : LayerAbstraction VariablesAPI.State StatDbAPI.State :=
+    {| abstraction := statdb_abstraction; |}.
 
   Example abstr_1_ok : statdb_abstraction (VariablesAPI.mkState 0 0) nil.
   Proof. unfold statdb_abstraction; auto. Qed.
@@ -77,6 +75,7 @@ Module StatDB (v : VarsAPI) <: StatDbAPI.
   (* END *)
   (* STUB: Admitted. *)
 
+(*
   Theorem init_ok : init_abstraction init abstr inited.
   Proof.
     eapply then_init_compose; eauto.
@@ -98,15 +97,30 @@ Module StatDB (v : VarsAPI) <: StatDbAPI.
     unfold statdb_abstraction, inited.
     intuition auto.
   Qed.
+*)
+
+
+  Theorem op_ok : forall opT T State (op : opT T) op_step,
+    proc_spec (fun (_ : unit) (state : State) =>
+      {|
+        pre := True;
+        post := fun (r : T) state' => op_step T op state r state';
+      |}) (Op opT T op) op_step.
+  Proof.
+    unfold proc_spec; intros.
+    inversion H0; subst; repeat sigT_eq.
+    simpl in *; eauto.
+  Qed.
+
+  Hint Resolve op_ok.
+
 
   (** ** Exercise : complete the proof of [add] *)
-  Theorem add_ok : forall v, proc_spec (add_spec v) (add v) abstr.
+  Theorem add_ok : forall v, proc_spec (spec_lower (add_spec v) abs) (add v) VariablesAPI.op_step.
   Proof.
     unfold add.
     intros.
 
-    apply spec_abstraction_compose; simpl.
-  (* SOL *)
     step_proc_basic; intros.
     destruct a'; simpl in *; intuition idtac.
     exists tt; simpl; intuition idtac.
@@ -127,18 +141,26 @@ Module StatDB (v : VarsAPI) <: StatDbAPI.
 
     eexists; intuition auto.
     unfold statdb_abstraction in *; simpl in *.
+
+    inversion H0; clear H0.
+    inversion H1; clear H1.
+    inversion H2; clear H2.
+    inversion H3; clear H3.
+
+    subst; repeat sigT_eq.
+    simpl in *.
+    deex. simpl in *.
+
     intuition omega.
   Qed.
   (* END *)
   (* STUB: Admitted. *)
 
   (** ** Exercise : complete the proof of [mean] *)
-  Theorem mean_ok : proc_spec mean_spec mean abstr.
+  Theorem mean_ok : proc_spec (spec_lower mean_spec abs) mean VariablesAPI.op_step.
   Proof.
     unfold mean.
     intros.
-
-    apply spec_abstraction_compose; simpl.
 
   (* SOL *)
     step_proc_basic; intros.
@@ -153,8 +175,13 @@ Module StatDB (v : VarsAPI) <: StatDbAPI.
       simpl in *; intuition subst.
 
       unfold statdb_abstraction in *.
-      destruct s; intuition; simpl in *; try congruence.
-      exists nil; intuition auto.
+      deex.
+      inversion H0; clear H0. simpl in *.
+      subst; repeat sigT_eq. intuition subst.
+      eexists.
+
+      intuition idtac. eauto. eauto.
+      destruct state1; intuition; simpl in *; try congruence.
 
     - step_proc_basic; intros.
       exists tt; simpl; intuition idtac.
@@ -165,22 +192,21 @@ Module StatDB (v : VarsAPI) <: StatDbAPI.
       simpl in *; intuition subst.
 
       unfold statdb_abstraction in *.
-      destruct s; intuition.
 
-      eexists; intuition auto.
+      inversion H0; clear H0.
+      inversion H1; clear H1.
+      subst; repeat sigT_eq. simpl in *. intuition subst.
+      deex.
+
+      destruct state; intuition.
+      simpl in *.
+
+      eexists; intuition auto. eauto. eauto.
       right.
       intuition ( try congruence ).
+      subst. simpl in *. eauto.
   Qed.
   (* END *)
   (* STUB: Admitted. *)
 
 
-End StatDB.
-
-
-Require Import VariablesImpl.
-Module StatDBImpl := StatDB Vars.
-Print Assumptions StatDBImpl.abstr_2_nok.
-Print Assumptions StatDBImpl.abstr_3_ok.
-Print Assumptions StatDBImpl.add_ok.
-Print Assumptions StatDBImpl.mean_ok.
