src/Spec/ProcTheorems.v
@@ -10,8 +10,8 @@ Require Import Proc.
 Ltac inv_exec' H :=
   inversion H; subst; clear H; repeat sigT_eq.
 
-Theorem exec_ret : forall T (v:T) w r,
-    exec (Ret v) w r ->
+Theorem exec_ret : forall opT State Sem T (v:T) w r,
+    @exec opT State Sem _ (Ret v) w r ->
     match r with
     | Finished v' w' => v = v' /\ w = w'
     end.
@@ -22,16 +22,16 @@ Qed.
 
 Ltac inv_ret :=
   match goal with
-  | [ H: exec (Ret _) _ _ |- _ ] =>
+  | [ H: exec _ (Ret _) _ _ |- _ ] =>
     apply exec_ret in H; safe_intuition; subst
   end.
 
 Ltac inv_exec :=
   match goal with
   | _ => inv_ret
-  | [ H: exec (Bind _ _) _ _ |- _ ] =>
+  | [ H: exec _ (Bind _ _) _ _ |- _ ] =>
     inv_exec' H; repeat inv_ret
-  | [ H: exec _ _ _ |- _ ] =>
+  | [ H: exec _ _ _ _ |- _ ] =>
     inv_exec' H; repeat inv_ret
   end.
 
@@ -45,32 +45,33 @@ we're proving that exec treats procedures up to the monad laws as equivalences
 between procedures).
  *)
 
-Definition exec_equiv T (p: proc T) p' :=
-  forall w r, exec p w r <-> exec p' w r.
+Definition exec_equiv {opT T State} Sem (p: proc opT T) p' :=
+  forall w r, @exec opT State Sem _ p w r <-> @exec opT State Sem _ p' w r.
 
-Instance exec_equiv_equiv T : Equivalence (exec_equiv (T:=T)).
+Instance exec_equiv_equiv opT State Sem T : Equivalence (@exec_equiv opT T State Sem).
 Proof.
   constructor; hnf; unfold exec_equiv; intros;
     repeat match goal with
-           | [ H: forall (w:world) (r: Result T), _,
-                 w: world,
-                 r: Result T |- _ ] =>
+           | [ H: forall (w:State) (r: Result State T), _,
+                 w: State,
+                 r: Result State T |- _ ] =>
              specialize (H w r)
            end; intuition.
 Qed.
 
-Theorem monad_left_id : forall T T' (p: T' -> proc T) v,
-    exec_equiv (Bind (Ret v) p) (p v).
+Theorem monad_left_id : forall opT T T' State Sem (p: T' -> proc opT T) v,
+    @exec_equiv _ _ State Sem (Bind (Ret v) p) (p v).
 Proof.
   unfold exec_equiv; split; intros.
   - inv_exec; eauto.
   - eapply ExecBindFinished; eauto.
 Qed.
 
-Theorem monad_assoc : forall `(p1: proc T)
-                        `(p2: T -> proc T')
-                        `(p3: T' -> proc T''),
-    exec_equiv (Bind (Bind p1 p2) p3) (Bind p1 (fun v => Bind (p2 v) p3)).
+Theorem monad_assoc : forall opT State Sem
+                        `(p1: proc opT T)
+                        `(p2: T -> proc opT T')
+                        `(p3: T' -> proc opT T''),
+    @exec_equiv _ _ State Sem (Bind (Bind p1 p2) p3) (Bind p1 (fun v => Bind (p2 v) p3)).
 Proof.
   unfold exec_equiv; split; intros.
   - destruct r; repeat (inv_exec; eauto).
