src/Lab1/VariablesImpl.v
@@ -8,20 +8,8 @@ Require Import VariablesAPI.
 
 Extraction Language Haskell.
 
-Module Vars <: VarsAPI.
-
-  Axiom init : proc InitResult.
-  Axiom read : var -> proc nat.
-  Axiom write : var -> nat -> proc unit.
-
-  Axiom abstr : Abstraction State.
-
-  Axiom init_ok : init_abstraction init abstr inited_any.
-  Axiom read_ok : forall v, proc_spec (read_spec v) (read v) abstr.
-  Axiom write_ok : forall v val, proc_spec (write_spec v val) (write v val) abstr.
-
-End Vars.
-
+(*
 Extract Constant Vars.init => "Variables.Ops.init".
 Extract Constant Vars.read => "Variables.Ops.read".
 Extract Constant Vars.write => "Variables.Ops.write".
+*)
